examples

examples/FunctorExamples/RobMarshallingExample.i.dfy
@@ -4,6 +4,11 @@ abstract module Marshalling {
 
 abstract module IntegerMarshalling refines Marshalling {
   type Thing = int
+
+  predicate intDiddle(foo: int, bar: Thing)
+  {
+    foo == bar
+  }
 }
 
 module Uint32Marshalling refines IntegerMarshalling {
@@ -12,11 +17,60 @@ module Uint32Marshalling refines IntegerMarshalling {
 abstract module SeqMarshalling(ElementMarshalling : Marshalling)
 {
   type Booger
+  predicate smDoodle(foo: ElementMarshalling.Thing) {
+    true
+  }
 }
 
-abstract module IntegerSeqMarshalling(IM : IntegerMarshalling) refines SeqMarshalling(IntegerMarshalling)
+module SeqMarshalling_applied_IntegerMarshalling
 {
-  type Doo = ElementMarshalling.Thing
+    import ElementMarshalling = IntegerMarshalling
+}
+
+module X {
+    import SeqMarshalling(IntegerMarshalling)
+}
+
+module Y {
+    import IM : IntegerMarshalling
+    import F = SeqMarshalling(IM)
+    predicate A(a: F.ElementMarshalling.Thing) { true }
+}
+
+module Z {
+    import IM : IntegerMarshalling
+    import G = SeqMarshalling(IM)
+    import Y
+    predicate A(a: G.ElementMarshalling.Thing) { Y.A(a) }
+}
+
+// So we know IM is the 1st parameter to SeqMarshalling, but we don't know which of SeqMarshalling's
+// import:'s it refers to.
+abstract module IntegerSeqMarshalling(IM : IntegerMarshalling) refines SeqMarshalling(IM)
+{
+  import IntegerMarshalling
+  // ElementMarshallinng is IM, which is known to be an IntegerMarshalling. So Thing = int now, right?
+  // I think I need to change SeqMarshalling to point to SeqMarshallingIM, in which ElementMarshalling has
+  // been replaced with IntegerMarshalling.
+  type Doo = IM.Thing
+  predicate pick(booger: Booger) {
+    true
+  }
+
+  predicate diddle(foo: int, bar: IntegerMarshalling.Thing)
+  {
+    && IM.intDiddle(foo, bar)
+    && smDoodle(bar)    // smDoodle comes from SeqMarshalling_applied, which has had ElementMarshalling replaced with IM, right?
+    && foo == bar
+  }
+
+  predicate daddle(foo: int, bar: Doo)
+  {
+    foo == bar
+  }
+
+  predicate dee(doo: Doo)
+  { true }
 }
 
 //module Uint32SeqMarshalling refines IntegerSeqMarshalling(Uint32Marshalling)
