examples/FastMarshalling.i.dfy
@@ -1,0 +1,74 @@
+include "../lib/Lang/NativeTypes.s.dfy"
+include "../lib/Lang/LinearSequence.i.dfy"
+
+import opened NativeTypes
+import opened LinearSequence_s
+import opened LinearSequence_i
+
+function interp_word(bs:seq<byte>) : (v:uint32)
+    requires |bs| == 4
+
+function as_word(bs:seq<byte>, offset:nat) : (v:uint32)
+    requires 0 <= offset <= |bs|-4
+    ensures v == interp_word(bs[offset..offset+4])
+
+method extract_word(shared bs:seq<byte>, offset:nat) returns (v:uint32)
+    requires 0 <= offset <= |bs|-4
+    ensures v == as_word(bs, offset)
+
+method replace_word(linear inout bs:seq<byte>, offset:nat, v:uint32) returns ()
+    requires 0 <= offset <= |old_bs|-4
+    ensures |bs| == |old_bs|
+    ensures forall i | 0<=i<offset || offset+4<=i<|old_bs| :: bs[i]==old_bs[i]
+    ensures as_word(bs, offset) == v;
+
+method entire_file() returns (linear v:seq<byte>)
+    ensures |v|>=8192;
+
+method read_page(shared v1: seq<byte>, page:nat) returns (linear v2:seq<byte>)
+    requires |v1|>=(page+1)*4096;
+    ensures v2[..] == v1[page*4096..(page+1)*4096];
+
+method discard<T>(linear v:T) returns ()
+
+method main() {
+    linear var orig_raw_data:seq<byte> := entire_file();
+    linear var offset_raw_data:seq<byte> := read_page(orig_raw_data, 1);
+    var orig_word:uint32 := extract_word(orig_raw_data, 4100);
+    var offset_word:uint32 := extract_word(offset_raw_data, 4);
+    calc {
+        orig_raw_data[..][4100..4104];
+        {   // having some extensionality troubles.
+            var x:= orig_raw_data[..];
+//            assert 4100==4096+4;
+//            assert 4104==4096+8;
+//            assert |x[4100..4104]| == 4 == |x[4096..8192][4..8]|;
+            assert forall i | 0<=i<4 ::
+                x[4100..4104][i] == x[4096..8192][4..8][i];
+            assert x[4100..4104] == x[4096..8192][4..8];
+        }
+        orig_raw_data[..][4096..8192][4..8];
+        offset_raw_data[..][4..8];
+    }
+    calc {
+        orig_word;
+        as_word(orig_raw_data[..], 4100);
+        as_word(offset_raw_data[..], 4);
+        offset_word;
+    }
+    var new_word:uint32;
+    assert as_word(orig_raw_data, 4100) == orig_word;
+    ghost var snap := orig_raw_data[..];
+    assert snap[4100..4104] == orig_raw_data[4100..4104];
+    replace_word(inout orig_raw_data, 4104, new_word);
+    assert snap[4100..4104] == orig_raw_data[4100..4104];
+    assert as_word(orig_raw_data, 4100) == orig_word;
+    assert as_word(orig_raw_data, 4104) == new_word;
+    discard(orig_raw_data);
+    discard(offset_raw_data);
+}
+
+/*
+FastMarshalling.i.dfy(30,0): Error: linear variable offset_raw_data must be unavailable at end of block
+FastMarshalling.i.dfy(30,0): Error: linear variable _v0 must be unavailable at end of block
+*/
