examples/FastMarshalling2.i.dfy
@@ -1,0 +1,229 @@
+include "../lib/Lang/NativeTypes.s.dfy"
+include "../lib/Lang/LinearSequence.i.dfy"
+
+import opened NativeTypes
+import opened LinearSequence_s
+import opened LinearSequence_i
+
+function interp_word(bs:seq<byte>) : (v:uint32)
+    requires |bs| == 4
+
+function as_word(bs:seq<byte>, offset:nat) : (v:uint32)
+    requires 0 <= offset <= |bs|-4
+    ensures v == interp_word(bs[offset..offset+4])
+
+method extract_word(shared bs:seq<byte>, offset:nat) returns (v:uint32)
+    requires 0 <= offset <= |bs|-4
+    ensures v == as_word(bs, offset)
+
+method replace_word(linear inout bs:seq<byte>, offset:nat, v:uint32) returns ()
+    requires 0 <= offset <= |old_bs|-4
+    ensures |bs| == |old_bs|
+    ensures forall i | 0<=i<offset || offset+4<=i<|old_bs| :: bs[i]==old_bs[i]
+    ensures as_word(bs, offset) == v;
+
+/*
+Given a seq of given length, you can extract a record from it.
+A datatype is a sum record. First byte(?) tells size of the rest.
+A constructor is a product record. Size may be variable, yes?
+
+datatype Point = Point(x:uint32, y:uint32)
+datatype Color = Red | Blue
+datatype Path = Path(id:uint32, pts:seq<Point>, color:Color)
+
+// I'd like to be able to say:
+// var offset,length := pointerMath(
+method extractPoint() returns (point: Point)
+
+No this is all nonsense. To use partial-reads of big datatypes,
+we really have to plan carefully what granularity of I/O we want to do,
+not bake it into the marshalling framework.
+*/
+
+/*
+So let's try to do something concrete.
+We should really have a Node "interface":
+    - one implemented by datatype Node
+    - another implemented by a NodeView object that contains
+        a NodeHeader
+        and some pointers to buffers
+        and has requireses that explain which methods you can call
+            based on which buffers are available.
+methods, then:
+    getPivotTable() -- accessor
+    getChildren() -- accessor. Maybe roll these together into getting a header object?
+    getBucketHeader(i)
+    getBucketMessageLocation(i, key)
+    getBucketMessage(i, key)
+...oh, we want to pull the indices for the buckets into the header block,
+too.
+    
+datatype NodeHeader = NodeHeader(
+    pivotTable:Pivots.PivotTable,
+    children:Option<seq<BT.G.Reference>>,   // why option, vs empty list?
+    bucketOffsets:seq<uint32>)
+method size(o:NodeHeader) returns (size:uint32)
+
+Should probably begin this conversation with just a Bucket for now.
+
+VBucket.getNumPairs() : int
+VBucket.getMessage(key: Key) : Option<Message>
+    requires VBucket.offsetAvailable(VBucket.offsetForKey(key: Key))
+VBucket.offsetForKey(key: Key)
+
+*/
+
+Okay, what would we do in C?
+
+Space-optimal, preserving nesting:
+struct Node {
+    struct Index {
+        // populated at load time by walking structures and counting up lengths
+        PivotTable *pivotTable;
+        ChildTable *childTable;
+        BucketIndexTable *bucketIndexTable;
+        BucketContentsTable *bucketContentsTable;
+    } index[0];
+    struct PivotTable {
+        uint32 pivotCount;
+        struct Pivot { Key key } pivots[];
+    }
+    struct ChildTable {
+        uint32 childCount;
+        struct Child { Reference ref } children[];
+    }
+    // We pretty much have to split the bucket data structure in half,
+    // to keep the keys all together at the beginning.
+    struct BucketIndexTable {
+        uint32 bucketCount;
+        struct BucketIndex {
+            uint32 keyCount;
+            Key keys[];
+        } buckets[];
+    }
+    struct BucketContentsTable {
+        uint32 bucketCount; // duplicates index info
+        struct BucketContents {
+            uint32 messageCount;  // duplicates index info
+            Message messages[];
+        } buckets[];
+    }
+}
+and then we'd have a function that computes the (offset==0,size) of the first
+load (everything except the bucket contents table), and another that computes
+same for messages in BucketContentsTable.
+
+Unmarshalling-optimal would marshall the offsets into the data structure so
+they don't need to be computed after the read by summing lengths.
+struct Node {
+    struct Offsets {
+        uint32 pivotTable;
+        uint32 childTable;
+        uint32 bucketIndexTable;
+        uint32 bucketContentsTable;
+    }
+    struct PivotTable {
+        uint32 pivotCount;  // could be computed from offsets, but why?
+        struct Pivot { Key key } pivots[];
+    }
+    struct ChildTable {
+        uint32 childCount;  // could be computed from offsets, but why?
+        struct Child { Reference ref } children[];
+    }
+    // We pretty much have to split the bucket data structure in half,
+    // to keep the keys all together at the beginning.
+    struct BucketIndexTable {
+        uint32 bucketCount;
+        struct BucketIndex {
+            uint32 keyCount;
+            uint32 bucketContentsOffset;    // offset from Node* to struct BucketContents
+            Key keys[];
+        } buckets[];
+    }
+    struct BucketContentsTable {
+        uint32 bucketCount; // duplicates index info, and not actually used.
+        struct BucketContents {
+            uint32 messageCount;  // duplicates index info, and not actually used.
+            Message messages[];
+        } buckets[];
+    }
+}
+
+findMessage(Node* node, Key* key) {
+    // All this stuff can be looked up if the Node "header" section is
+    // all available.
+    PivotTable* pivotTable = (((void*) node) + node.offsets.pivotIndexTable);
+    BucketIndexTable* bucketIndexTable =
+        (BucketIndexTable*) (((void*) node) + node.offsets.bucketIndexTable);
+    BucketContentsTable* bucketContentsTable =
+        (BucketContentsTable*) (((void*) node) + node.offsets.bucketContentsTable);
+
+    bucketNum = pivotTable.findBucket(key);
+    // ignore child lookup for now; it can be done from the header.
+
+    BucketIndex* bi = bucketIndexTable.buckets[bucketNum];
+    // This thing does a binary search using keys[],
+    // then uses bucketContentsOffset to pointer-math (offset, size)
+    // of desired Message*.
+    DataAddress messageAddress = bi->getMessagePointer(key);
+
+    // May span multiple pages. This function checks if the pages we need
+    // are cached; if not, it does an IO to fetch them.
+    cache->pageIn(messageAddress);
+
+    // NOTE: What's the cache architecture for the Node index sections?
+    // If they're bigger than a page, we have a contiguity problem.
+    // One possibly-simple strategy: allocate node indices as a different
+    // page size at disk-allocation-time. Eww.
+    // Splinter strategy (everything fits in 4k) starting to look pretty sweet.
+
+    // Copy the message out, to deal with possible crossing of a noncontiguous
+    // page boundary.
+    Message message = messageAddress.extract(cache);
+    return message;
+}
+
+Can we let the cache just fault stuff in? OS cache probably does clever
+prefetching if we're scanning, whereas we'd turn a scan into seek-synchronous
+IO party. Or have a heuristic for when to fault the whole Node in?
+
+something more ultra-integrated: A node is:
+    {
+        structured stuff that's guaranteed to fit in a page
+        bucket counts
+        pivot range
+        offset to key array
+        offset to message array
+    }
+    { key array } indexed into by pivot table, bucket tables
+    { message array } indexed into by bucket tables
+
+So a PivotView would know how to peek into one of these clever backing store
+thingies, as would a BucketView.
+
+So we'd do:
+findMessage(Node* integ, Key* key) {
+    Ans<uint32> bucketIdxAns = PivotView(cache, integ).findBucket(key);
+    // tries to bin-search the pivot table
+    if bucketIdxAns.fault? {
+        cache.fault(bucketIdxAns.faultReq);
+        return;
+    }
+
+    Ans<Message> msgAns = BucketView(cache, integ, bucketIdxAns.value).findMessage(key);
+    // Tries to bin-search the bucket keys, which get sorted near the
+    // beginning to maximize chance of colocating with other searches.
+    // Then tries to retrieve the message.
+    if msgAns.fault? {
+        cache.fault(msgAns.faultReq);
+        return;
+    }
+    // if it works, it copies out the Message (to deal with contiguity).
+    return msgAns.value;
+}
+
+Ans<Message> BucketView.findMessage()
+{
+    // binsearch proceeds with Ans<Key> key
+    produces message idnex
+}
