examples/FastMarshalling3.i.dfy
@@ -1,0 +1,38 @@
+include "../lib/Lang/NativeTypes.s.dfy"
+include "../lib/Lang/LinearSequence.i.dfy"
+include "../lib/MarshalledAccessors.i.dfy"
+
+method findPivotIdx(mnode: MarshalledNode, key:Key) returns (idx:nat)
+{
+    return binarySearch(mnode.pivots(), key);
+}
+
+method findChildRef(mnode: MarshalledNode, key:Key)
+{
+    var idx := findPivotIndex(mnode, key);
+    var mChildTable := mnode.childTable();
+    var childRef := mChildTable.Element(idx);
+    return childRef;
+}
+
+method findMessage(mnode: MarshalledNode, key:Key) returns Option<Message>
+{
+    var idx := findPivotIndex(mnode, key);
+    var mKeyTable := mnode.keyTable();
+    var keyIdx := binarySearch(mnode.pivots(), key);
+    if mKeyTable.Element(keyIdx) != key {
+        return None
+    }
+    var mValueTable := mnode.valueTable();
+    var ...now we're back to trying to assemble pieces. I like Rob's idea
+    of going with the Splinter tables.
+    var childRef := mChildTable.Element(idx);
+}
+
+method LookupExample()
+{
+    // TODO we need a way for a MarshalledNode to work even if it can
+    // only see a subset of the data!
+    var nodePrefixData := Read(nodeStartAddress, 4096);
+    var mnode := MarshalledNode(nodePrefixData, 0);
+}
