examples/FastMarshalling4.i.dfy
@@ -1,0 +1,67 @@
+include "../lib/Lang/NativeTypes.s.dfy"
+include "../lib/Lang/LinearSequence.i.dfy"
+include "../lib/MarshalledAccessors.i.dfy"
+
+// Can we rely on a global invariant that LBAs contain the type of
+// block expected of them by references to them?
+
+// Also, references are accounted at allocation-unit granularity,
+// not IO/unit granularity. Are we changing how we do the indirection
+// table, now that it's got 64X the number of entries? I guess not yet;
+// we'll leave the allocation unit big for now.
+
+datatype TrunkNode {
+  pivots: seq<Key>,
+  children: seq<LBA>,
+  branches: seq<LBA>
+}
+
+predicate WFTrunkNode(n:TrunkNode) {
+  |n.pivots| + 1 == |n.children| == |n.branches|
+}
+
+datatype BranchIndexNode {
+  pivots: seq<Key>,
+  children: seq<LBA>
+}
+
+predicate WFBranchIndexNode(n:BranchIndexNode) {
+  |n.pivots| + 1 == |n.children|
+}
+
+datatype BranchLeafNode {
+  pivots: seq<Key>,
+  messages: seq<Message>
+}
+
+predicate WFBranchLeafNode(n:BranchLeafNode) {
+  |n.pivots| + 1 == |n.messageschildren|
+}
+
+datatype Block = TrunkNodeBlock(t:TrunkNode) | BranchIndexNodeBlock(b:BranchIndexNode) | BranchLeafNodeBlock(l:BranchLeafNode)
+
+datatype ReadOp = ReadOp(ref:LBA, block:Block)
+
+type BtreeLayer = ReadOp
+type BtreeLookup = seq<BtreeLayer>
+datatype Layer = Layer(trunk: ReadOp, btree: BtreeLookup)
+type Lookup = seq<Layer>
+
+predicate WFBtreeLookup(bl: BtreeLookup) {
+    && |bl| > 0
+    && Last(bl).block.BranchLeafNodeBlock?
+    && (forall i | 0<=i<|bl|-1 :: bl[i].block.BranchIndexNodeBlock?)
+    // the triggery part we gotta hide
+    && (forall i | 0<=i<|bl|-1 ::
+        var slot := FindSlot(bl[i].block.b.pivots);
+        && bl[i].block.b.children[slot] == bl[i+1].ref)
+}
+
+predicate WFLookup(l: Lookup) {
+    && |l|>0
+    && Last(l)
+}
+
+// And then I guess the impl is the first place where we use Marshalled*
+// versions of these data structures. We argue that we have a Lookup by
+// defending the Blocks they support.
