examples/FunctorExamples/CommonApplication.i.dfy
@@ -1,0 +1,91 @@
+abstract module A {
+  datatype T = T
+}
+
+module B refines A {
+}
+
+abstract module C(a: A) {
+}
+
+abstract module D(a: A) refines C(a) {
+}
+
+// { D -> PM{D's literals + a -> AM(A), ptr to C(a)'s AM-mod-syms }
+
+abstract module E(c: C) {
+    type R
+}
+
+// { E -> PM(
+
+abstract module F(e: E) {
+}
+
+abstract module G(a: A) refines E(C(a)) {
+    import X = a
+    import Y = c.a
+    import Z = E(C(a)).c.a
+    lemma types_eq(x:X.T, y:Y.T, z:Z.T, r:R)
+    requires x == y == z
+    {}
+}
+
+abstract module H(a: A) refines F(G(a)) {
+  import X = a
+  // > I think "import e.c.a" is impossible ...
+  // It's fine now that we have paved the module parts of the Resolver
+  // and replaced it with the ModuleResolver.
+  import U = e.c.a
+  import Y = G(a).a
+  import Z = C(a).a
+  import W = G(a).c.a
+  import V = F(G(a)).e.c.a
+
+  lemma types_eq(x: X.T, y: Y.T, z: Z.T, w: W.T, v: V.T)
+  requires /*x == y == */ z == w == v
+  {
+  }
+}
+
+///////////////////////////////////////////////////////////////////////////
+//
+//module Key {
+//    type KeyType
+//}
+//
+//module IntKey refines Key {
+//    type KeyType = int
+//}
+//
+//module A(km:Key) {
+////    type T = List<km.KeyType>
+//    datatype T = Foo(k : km.KeyType)
+//}
+//
+//module B(km:Key) {
+//    import A = A(km)
+//    predicate empty(thing: A.T) { |thing| == 0 }
+//}
+//
+//module C(km:Key) {
+//    import B = B(km)
+//    predicate fuzzy(thing: B.A.T) { B.empty(thing) }
+//    // AM: thing has type A.Foo<UserDefinedType>
+//}
+//
+//module C2 {  // should name-mangle this C_O_module_DD_DIntKey_C
+//    import km = IntKey
+//    import B = B(km)
+//    predicate fuzzy(thing: B.A.T) { B.empty(thing) }
+//    // AM: thing has type A.Foo<UserDefinedType>
+//}
+//
+//
+//module D {
+//    import C = C(IntKey)
+//    // thing has type List<int>
+//    // In this AM, this is the first time A(IntKey).T has been instantiated;
+//    // it's a new datatype (with k:int) that's not been seen before.
+//    // AM: thing has type A.Foo<UserDefinedType>
+//}
