examples/FunctorExamples/CommonApplicationClassic.i.dfy
@@ -1,0 +1,25 @@
+module ABase {
+    type Key
+}
+
+module InnocentA refines ABase {
+    type Key = int
+}
+
+module SinisterA refines ABase {
+    type Key = bool
+}
+
+abstract module P {
+    import A : ABase
+}
+
+abstract module B {
+    module P1def refines P { import A = InnocentA }
+    import P1 = P1def
+    module P2def refines P { import A = SinisterA }
+    import P2 = P2def
+    lemma foo(a: P1.A.Key, b: P2.A.Key)
+        ensures a == b
+    { }
+}
