examples/FunctorExamples/DottyDot.i.dfy
@@ -1,0 +1,13 @@
+module A {
+    predicate x() { true }
+}
+
+module B {
+    import A1 = A
+    import A2 = A
+}
+
+module C {
+    import B
+    predicate x() { B.A1.x() }
+}
