examples/FunctorExamples/RefineWithRefinement.i.dfy
@@ -1,0 +1,21 @@
+abstract module Marshalling {
+  type Thing
+}
+ 
+abstract module IntegerMarshalling refines Marshalling {
+  type Thing = int
+}
+ 
+abstract module SeqMarshalling
+{
+  import ElementMarshalling : Marshalling
+}
+
+abstract module IntegerSeqMarshalling refines SeqMarshalling
+{
+  import IM : IntegerMarshalling
+  import ElementMarshalling = IM
+  predicate x(a:int) { true }
+  predicate y(b:ElementMarshalling.Thing) { x(b) }
+}
+
