examples/FunctorExamples/RefinementNaming.i.dfy
@@ -1,0 +1,8 @@
+
+abstract module E {
+  type R
+}
+
+abstract module G refines E {
+  predicate foo(r:R) { false }
+}
