examples/FunctorExamples/RefinementScope.i.dfy
@@ -1,0 +1,9 @@
+module A {
+    type T // UserDataType
+}
+abstract module E(ea:A) {
+//abstract module E { import ea : A
+  predicate f1(x:ea.T) { false }
+}
+abstract module G(ga:A) refines E(ga) { }
+//abstract module G refines E { }
