examples/FunctorExamples/SimpleModuleApplication.i.dfy
@@ -1,0 +1,27 @@
+module A {
+    type T // UserDataType
+}
+module A' refines A {
+    type T = int    // TypeSynonym
+}
+module E(ea: A) {
+  predicate f1(x:ea.T) { false }
+}
+module F {
+    import Aalias = A
+    import EA' = E(A')
+        // 1. construct a ModuleDefinition right here at the point of Application -- and ask the Resolver to resolve it?
+        // 2. You've already done resolution for E; do some translation of the type resolution for E(A')
+    predicate f2(x:EA'.ea.T) ensures false {
+        x < 7
+    }
+}
+
+module G(ga: A) refines E(ga) {
+}
+module H(ha: A) refines G(ha) {
+  import U=ea
+  import V=G(ha).ea
+  import W=E(ha).ea
+  predicate f3(x:U.T) ensures false { false }
+}
